theories/security.v
@@ -5,6 +5,7 @@ Require Import Unicode.Utf8.
 
 Require Import config.
 Require Import data_model.
+Require Import expression.
 Require Import lattice.
 Require Import relation.
 Require Import semantics.
@@ -44,13 +45,17 @@ Inductive join_ok: Policy.policy → trace_ty → trace_ty → Prop :=
 .
 
 (*
- * The dependency graph:
- *
- * label_transition_valid --> label_transition_valid_impl --> valid_transition
- *  ^                                                               |
- *  |                                                               |
- *  +---------------------------------------------------------------+
+ * Checks against for each element, can it be released via the current label?
  *)
+Inductive
+valid_transition: prov_type → Policy.policy → trace_ty → Prop :=
+  | ValidEmpty: ∀ prov lbl, valid_transition prov lbl ∅
+  | ValidTransition: ∀ prov lbl lbl' tr,
+      lbl' = extract_policy tr →
+      lbl =[ prov ]=> lbl' →
+      valid_transition prov lbl tr
+.
+
 Inductive label_transition_valid: trace_ty → Prop :=
   | LabelTransitionTrEmpty: label_transition_valid ∅
   | LabelTransitionTrLinear: ∀ tr prov lbl l,
@@ -74,16 +79,6 @@ label_transition_valid_impl: prov_type → Policy.policy → list (trace_ty) →
       label_transition_valid_impl prov lbl tl →
       valid_transition prov lbl hd →
       label_transition_valid_impl prov lbl (hd :: tl)
-(*
- * Checks against for each element, can it be released via the current label?
- *)
-with
-valid_transition: prov_type → Policy.policy → trace_ty → Prop :=
-  | ValidEmpty: ∀ prov lbl, valid_transition prov lbl ∅
-  | ValidTransition: ∀ prov lbl lbl' tr,
-      lbl' = extract_policy tr →
-      lbl =[ prov ]=> lbl' →
-      valid_transition prov lbl tr
 .
 
 (*
@@ -99,6 +94,18 @@ Inductive trace_ok: trace → Prop :=
       trace_ok tl →
       trace_ok (hd :: tl)
 .
+
+Lemma label_lookup_no_effect: ∀ tr id item,
+  trace_ok tr →
+  label_lookup tr id = Some item →
+  label_transition_valid item.
+Proof.
+  induction tr.
+  - discriminate.
+  - intros. destruct a. simpl in H0. destruct (Nat.eqb id n) eqn: Hn.
+    + inversion H0; subst. inversion H; subst. auto.
+    + eapply IHtr; eauto. inversion H; subst. auto.
+Qed.
 
 Lemma database_get_contexts_trace_ok: ∀ db s r n Γ β tr,
   database_get_contexts db n = Some (RelationWrapped s r, Γ, tr, β) →
@@ -149,20 +156,119 @@ Proof.
       * apply IHtr1. assumption. assumption.
 Qed.
 
+Lemma eval_ok: ∀ n in_agg Γ Γ' β β' tr tr' tp tp' gb gb' expr v,
+  trace_ok tr →
+  eval n expr in_agg ((Γ, β), tr, tp, gb) (Some (((Γ', β'), tr', tp', gb', v))) →
+  trace_ok tr'.
+Proof.
+Admitted.
+
+Lemma eval_expr_in_relation_ok: ∀ s r ty r' Γ Γ' β β' tr tr' expr,
+  trace_ok tr →
+  eval_expr_in_relation s r ty Γ β tr expr (Some (r', Γ', β', tr')) →
+  trace_ok tr'.
+Proof.
+  induction r; intros; inversion H0; subst;
+  try discriminate; intuition;
+  inversion H10; try inversion H1; subst; try discriminate.
+  - inversion H9. subst. apply inj_pair2_eq_dec in H26. subst.
+    + eapply IHr; eauto.
+    + apply basic_type_eq_dec.
+  - inversion H9. inversion H29. subst. eapply IHr; eauto.
+  - inversion H9. subst. eapply IHr.
+    + apply eval_ok in H1. eapply H1. assumption.
+    + eauto.
+  - cheat. (* Let us do it later. *)
+Qed.
+
+Lemma join_policy_and_trace_ok: ∀ l1 l2 com Γ1 Γ2 Γ tr1 tr2 tr,
+  trace_ok tr1 →
+  trace_ok tr2 →
+  join_policy_and_trace l1 l2 com Γ1 Γ2 tr1 tr2 (Some (Γ, tr)) →
+  trace_ok tr.
+Proof.
+  induction l1; intros; inversion H1; subst;
+  try discriminate; try (apply trace_ok_merge_ok; auto).
+  inversion H4. inversion H5. subst. clear H4.
+  econstructor; eauto; simpl.
+  - inversion H21; subst. intuition.
+    eapply LabelTransitionTrBranch with (tr1 := tr1') (tr2 := tr2'); eauto.
+    + reflexivity.
+    + apply label_lookup_no_effect in H11; auto.
+    + apply label_lookup_no_effect in H12; auto.
+    + econstructor; eauto. 
+  - assert (trace_ok tl4) by (inversion H; subst; auto).
+    assert (trace_ok tl5) by (inversion H0; subst; auto).
+    eapply IHl1 with (tr1 := tl4) (tr2 := tl5); eauto.
+Qed.
+
+Lemma trace_ok_join_ok_aux: ∀ s1 s2 join_by t r rout Γ1 Γ2 Γ β1 β2 β tr1 tr2 tr,
+  trace_ok tr1 →
+  trace_ok tr2 →
+  relation_join_by_prv_helper s1 s2 join_by t r Γ1 Γ2 β1 β2 tr1 tr2 (Some (rout, Γ, β, tr)) →
+  trace_ok tr.
+Proof.
+  (* Induction follows the pattern of the inductive relation. *)
+  induction r; intros; inversion H1; subst.
+  - apply trace_ok_merge_ok; auto.
+  - apply inj_pair2_eq_dec in H2, H3, H4, H4, H4; subst.
+    + discriminate.
+    + apply list_eq_dec. apply Nat.eq_dec.
+    + apply list_eq_dec. apply attribute_eq_dec.
+    + apply list_eq_dec. apply attribute_eq_dec.
+    + apply list_eq_dec. apply attribute_eq_dec.
+    + apply list_eq_dec. apply attribute_eq_dec.
+  - apply inj_pair2_eq_dec in H2, H3, H4, H4, H4; subst.
+    + inversion H3; subst.
+      assert (trace_ok p_cons) by (eapply IHr with (tr1 := tr1) (tr2 := tr2); eauto).
+      eapply trace_ok_merge_ok with (tr1 := p_merged) (tr2 := p_cons); eauto.
+      eapply join_policy_and_trace_ok with (tr1 := tr1) (tr2 := tr2); eauto.
+    + apply list_eq_dec. apply Nat.eq_dec.
+    + apply list_eq_dec. apply attribute_eq_dec.
+    + apply list_eq_dec. apply attribute_eq_dec.
+    + apply list_eq_dec. apply attribute_eq_dec.
+    + apply list_eq_dec. apply attribute_eq_dec.
+Qed.
+
 Lemma trace_ok_join_ok: ∀ s1 s2 join_by r1 r2 r Γ1 Γ2 Γ β1 β2 β tr1 tr2 tr,
   trace_ok tr1 →
   trace_ok tr2 →
-  relation_join_by_prv s1 s2 join_by r2 r1 Γ2 Γ1 β2 β1 tr2 tr1 (Some (r, Γ, β, tr)) →
+  relation_join_by_prv s1 s2 join_by r1 r2 Γ1 Γ2 β1 β2 tr1 tr2 (Some (r, Γ, β, tr)) →
   trace_ok tr.
 Proof.
-Admitted.
+  induction r1; intros.
+  - inversion H1; subst; try constructor.
+    apply inj_pair2_eq_dec in H2.
+    + discriminate.
+    + apply list_eq_dec. apply attribute_eq_dec.
+  - inversion H1; subst; try constructor.
+    apply inj_pair2_eq_dec in H2, H3, H4, H4, H4; subst.
+    + inversion H2; subst.
+      assert (trace_ok p_cons) by (eapply IHr1 with (tr1 := tr1) (tr2 := tr2); eauto).
+      eapply trace_ok_merge_ok with (tr1 := p_hd) (tr2 := p_cons).
+      * apply trace_ok_join_ok_aux in H13; auto.
+      * assumption.
+    + apply list_eq_dec. apply Nat.eq_dec.
+    + apply list_eq_dec. apply attribute_eq_dec.
+    + apply list_eq_dec. apply attribute_eq_dec.
+    + apply list_eq_dec. apply attribute_eq_dec.
+    + apply list_eq_dec. apply attribute_eq_dec.
+Qed.
 
 Lemma trace_ok_proj_ok: ∀ s s' r r' Γ Γ' β β' t t' pl,
   trace_ok t →
   apply_proj_in_relation s s' r pl Γ β t (Some (r', Γ', β', t')) →
   trace_ok t'.
 Proof.
-Admitted.
+  induction s'; intros; inversion H0; subst; intuition.
+  - discriminate.
+  - inversion s_case. subst.
+    apply eval_expr_in_relation_ok in H9.
+    eapply IHs'.
+    + eapply H9.
+    + eauto.
+    + assumption.
+Qed.
 
 Lemma eval_predicate_in_relation_ok: ∀ s r Γ β t e r' Γ' β' t',
   trace_ok t →
@@ -325,8 +431,8 @@ Proof.
               ** eapply H3.
               ** reflexivity.
            ++ eapply trace_ok_join_ok.
-              ** eapply H6.
               ** eapply H.
+              ** eapply H6.
               ** eapply H3.
         -- left. eapply E_JoinError2.
            ++ eapply H5.
